Test/Nat/ZeroSub'.lean
@@ -3,5 +3,5 @@ import Smt
 example : ∀ x, 0 - x = 0 := by
   intro x
   induction x with
-  | zero => smt; rfl
-  | succ x ih => smt [ih]; simp [ih, Nat.sub_succ]
+  | zero => smt +trust
+  | succ x ih => smt +trust [ih]
