Test/Prop/ModusPonens.lean
@@ -1,4 +1,14 @@
 import Smt
 
-theorem modus_ponens {p q : Prop} : p → (p → q) → q := by
-  smt
+theorem modus_ponens (p q : Prop) (hp : p) (hpq : p → q) : q := by
+  smt +showQuery
+  exact hpq hp
+
+example (p q : Prop) (hp : p) (hpq : p → q) : q := by
+  smt [hp, hpq]
+
+example (p q : Prop) (hp : p) (hpq : p → q) : q := by
+  smt [*]
+
+example (p q : Prop) (hp : p) (hpq : p → q) : q := by
+  smt (timeout := .some 1) [*]
